\documentclass[12pt]{article}
\usepackage{amsmath}
\usepackage{amssymb}
\usepackage{graphicx}
\usepackage{hyperref}
\usepackage{multicol}
\usepackage[latin1]{inputenc}
\usepackage{listings}
\usepackage{scrextend}


% Used for code blocks ----------------------------------------------------------------
\usepackage{color}
\usepackage{xcolor}
\usepackage{listings}

\usepackage{caption}
\DeclareCaptionFont{white}{\color{white}}
\DeclareCaptionFormat{listing}{\colorbox{gray}{\parbox{\textwidth}{#1#2#3}}}
\captionsetup[lstlisting]{format=listing,labelfont=white,textfont=white}
% -----------------------------------------------------------------------------------------



\title{ComS 342\\Recitation 2, 10:00 Tuesday\\Homework 2}
\author{Sean Gordon}
%\date{09/09/2019}

\begin{document}
\maketitle


\noindent 1.\\
\indent (a) (let ((f 58)) (* (- f 32) (/ 5 9) ))\\\\
\indent (b) ( let( (x 12) (y 1) )( let( (x (- x 11)) )(- x y)))\\


\noindent 2.\\
\indent (a) This expression returns an error. The issue is in the second scope:\\
\indent \indent (let ((z 2) (x y)) (+ x z))\\
\indent \indent This can be evaluated as $\to$ (z = 2), (x = y), (x += z)\\
\indent \indent However, y is undefined here, so x = y is unable to be calculated.\\

\indent (b) This expression evaluates to 3. Procedure below:\\
\indent \indent \{x = 3, y = 0, \{y = (y = x)\}\} $\Rightarrow$ \{\{y = (y = 3)\}\} $\Rightarrow$ \{\{y = 3\}\} $\Rightarrow$ 3\\

\noindent 3.\\
\indent (a) Free: a, b\\
\indent \indent Bound: c, x, y, z\\

\indent (b) Free: b, c, g, y\\
\indent \indent Bound: a, x\\



%\begin{lstlisting}
%\end{lslisting}
\end{document}