\documentclass[12pt]{article}
\usepackage[12pt]{moresize}
\usepackage[margin=1in]{geometry}

\usepackage{amsmath}
\usepackage{amssymb}

\usepackage{graphicx}
\usepackage{subcaption}

\usepackage{multirow} %Combining rows in tables
\usepackage{diagbox}  %Table box split in twain
\usepackage{hhline}
\usepackage{makecell} 

\usepackage[ruled,linesnumbered]{algorithm2e}
\usepackage{algpseudocode}
\usepackage{alltt}

\usepackage{multicol}

\usepackage{amssymb} %\checkmark symbol

%\usepackage{hyperref}
%\usepackage[latin1]{inputenc}
%\usepackage{listings}
%\usepackage{scrextend}
%\usepackage{changepage} %Adjustwidth

 

\title{ComS 474\\Final Exam}
\author{Sean Gordon}
\date{Nov 26, 2020}

\begin{document}
\maketitle


\section{Regular Problems}
\ \\


\noindent 1) $
\begin{pmatrix}
1 & 1/2 & 1/2 \\
1/3 & 1/2 & 1
\end{pmatrix} * 
\begin{pmatrix}
0.5 & 1 & 6 \\
3 & -4 & 2
\end{pmatrix} = 
\begin{pmatrix}
0.5 & 0.5 & 3 \\
1 & -2 & 2
\end{pmatrix}$\\



\noindent \hrulefill \\



\noindent 2) 
(a) $
\begin{pmatrix}
1 & 1/2 & 1/2 \\
1/3 & 1/2 & 1
\end{pmatrix} * 
\begin{pmatrix}
0.5 & 3 \\
1 & -4 \\
6 & 2
\end{pmatrix} = 
\begin{pmatrix}
4 & 2 \\
6.667 & 1
\end{pmatrix}$\\\\

(b) $
\begin{pmatrix}
1 & 1/3 \\
1/2 & 1/2 \\
1/2 & 1
\end{pmatrix} * 
\begin{pmatrix}
0.5 & 1 & 6 \\
3 & -4 & 2
\end{pmatrix} = 
\begin{pmatrix}
4 & 6.667 \\
2 & 1
\end{pmatrix}$\\



\noindent \hrulefill \\



\noindent 3) $\left(
\begin{pmatrix}
1 & 1/3 \\
1/2 & 1/2 \\
1/2 & 1
\end{pmatrix} * 
\begin{pmatrix}
0.5 & 1 & 6 \\
3 & -4 & 2
\end{pmatrix}\right) + 1 \ \Rightarrow \
\begin{pmatrix}
4 & 6.667 \\
2 & 1
\end{pmatrix} + 1 = 
\begin{pmatrix}
5 & 7.667 \\
3 & 2
\end{pmatrix}$\\



\noindent \hrulefill \\



\noindent 4) $\hat y = \phi(w^Tx) = ((1/2)*2)^2+((1/3)*3)^2+((1/4)*4)^2+((1/5)*5)^2 = 4$\\[-.4em]



\noindent \hrulefill \\\pagebreak



\noindent 5) As $\hat y = (w^Tx)^2$...\\\\
\indent (a) {\Large $\frac{\partial E}{\partial \hat y}$} = {\Large $\frac{\partial (y + \hat y)}{\partial \hat y}$} = {\Large $\frac{\partial y}{\partial \hat y}$}+{\Large $\frac{\partial \hat y}{\partial \hat y}$} = 0+1 = $1$\\[.4em]

\indent (b) {\Large $\frac{\partial \hat y}{\partial w^Tx}$} = {\Large $\frac{\partial (w^Tx)^2}{\partial w^Tx}$} = {\Large $\frac{\partial (u)^2}{\partial u}$} = $2u$ = $2w^Tx$ =\\[.4em]
\indent \indent \ $2((1/2)*2)+2((1/3)*3)+2((1/4)*4)+2((1/5)*5) = 8$\\[.4em]

\indent (c) {\Large $\frac{\partial w^Tx}{\partial x_1}$} = {\Large $\frac{\partial (w_0x_0 + w_1x_1 + w_2x_2 + w_3x_3)}{\partial x_1}$} = $w_1$\\[.4em]

\indent (d) {\Large $\frac{\partial E}{\partial x_1}$} = {\Large $\frac{\partial E}{\partial \hat y}$} {\Large $\frac{\partial \hat y}{\partial w^Tx}$} {\Large $\frac{\partial w^Tx}{\partial x_1}$} = $1 * 8 * w_1$ = $1 * 8 * 3$ = 24\\[.4em]



\noindent \hrulefill \\



\noindent 6) \\
\indent (a) {\Large $\frac{\partial E}{\partial x}$} = $
\begin{pmatrix}
{\Large \frac{\partial E}{\partial x_0}}\\[.4em]
{\Large \frac{\partial E}{\partial x_1}}\\[.4em]
{\Large \frac{\partial E}{\partial x_2}}\\[.4em]
{\Large \frac{\partial E}{\partial x_3}}
\end{pmatrix} = 
\begin{pmatrix}
w_0 \\
w_1 \\
w_2 \\
w_3 
\end{pmatrix} = w = 
\begin{pmatrix}
2 \\
3 \\
4 \\
5 
\end{pmatrix}$\\[.4em]

\indent (b) {\Large $\frac{\partial E}{\partial w}$} = $
\begin{pmatrix}
{\Large \frac{\partial E}{\partial w_0}}\\[.4em]
{\Large \frac{\partial E}{\partial w_1}}\\[.4em]
{\Large \frac{\partial E}{\partial w_2}}\\[.4em]
{\Large \frac{\partial E}{\partial w_3}}
\end{pmatrix} = 
\begin{pmatrix}
x_0 \\
x_1 \\
x_2 \\
x_3 
\end{pmatrix} = x = 
\begin{pmatrix}
1/2 \\
1/3 \\
1/4 \\
1/5 
\end{pmatrix}$\\[.4em]



\noindent \hrulefill \\\pagebreak



\section{Bonus Problems}
\ \\


\noindent 7) $x^1 = \phi\left[
\begin{pmatrix}
1 & -1 & 0.1\\
1 & -1 & 0.1\\
1 & -1 & 0.1
\end{pmatrix}
\begin{pmatrix}
1\\ 1\\ 1
\end{pmatrix}\right]= max\left(
\begin{pmatrix}
0.1\\ 0.1\\ 0.1
\end{pmatrix}, 
\begin{pmatrix}
0\\ 0\\ 0
\end{pmatrix}\right) = 
\begin{pmatrix}
0.1\\ 0.1\\ 0.1
\end{pmatrix}$\\\\

\indent $x^2 = \phi\left[
\begin{pmatrix}
0.5 & 0.5 & 0.5 & 0.5\\
0.5 & 0.5 & 0.5 & 0.5
\end{pmatrix}
\begin{pmatrix}
1\\ 0.1\\ 0.1\\ 0.1
\end{pmatrix}\right]= max\left(
\begin{pmatrix}
0.65\\ 0.65
\end{pmatrix}, 
\begin{pmatrix}
0\\ 0
\end{pmatrix}\right) = 
\begin{pmatrix}
0.65\\ 0.65
\end{pmatrix}$\\\\

\indent $x^3 = \phi\left[
\begin{pmatrix}
0.25 & 0.25 & 0.25\\
0.25 & 0.25 & 0.25
\end{pmatrix}
\begin{pmatrix}
1\\ 0.65\\ 0.65
\end{pmatrix}\right]= max\left(
\begin{pmatrix}
0.575 \\ 0.575
\end{pmatrix}, 
\begin{pmatrix}
0\\ 0
\end{pmatrix}\right) = 
\begin{pmatrix}
0.575 \\ 0.575
\end{pmatrix}$\\



\noindent \hrulefill \\



\noindent 8) $\delta^{(3)} = \left(
\begin{pmatrix}
x_1^{(3)} \\ x_2^{(3)}
\end{pmatrix} - 
\begin{pmatrix}
y_1 \\ y_2
\end{pmatrix}\right)^2 = 
\begin{pmatrix}
(x_1^{(3)}y_1)^2 \\ (x_2^{(3)}y_2)^2
\end{pmatrix}$\\\\

\indent $\delta^{(2)} = 
\begin{pmatrix}
0(1 - 0) \\ 3.8(1 - 3.8) \\ 3.8(1 - 3.8)
\end{pmatrix} \circ \left(
\begin{pmatrix}
1 & 1 \\
1 & 1 \\
1 & 1 
\end{pmatrix}
\begin{pmatrix}
7.6 \\ 8.6
\end{pmatrix} \right) = 
\begin{pmatrix}
0 \\ -172.368 \\ -172.368
\end{pmatrix}
$\\\\

\indent $\delta^{(1)} = 
\begin{pmatrix}
0(1 - 0) \\ 0.3(1 - 0.3) \\ 0.3(1 - 0.3) \\ 0.3(1 - 0.3)
\end{pmatrix} \circ \left(
\begin{pmatrix}
2 & 2 \\
2 & 2 \\
2 & 2 \\
2 & 2 
\end{pmatrix}
\begin{pmatrix}
-172.368 \\ -172.368
\end{pmatrix}\right) = 
\begin{pmatrix}
0 \\ -144.789 \\ -144.789 \\ -144.789
\end{pmatrix}
$\\










\ \\\\\\\\\\



\noindent 9) $W^{(0)}: 3\times3$, \ $W^{(1)}: 4\times2$, \ $W^{(2)}: 3\times2$\\



\noindent \hrulefill \\



\noindent 10) $x^1 = \phi\left[
\begin{pmatrix}
0.1 & 0.1 & 0.1\\
0.1 & 0.1 & 0.1\\
0.1 & 0.1 & 0.1
\end{pmatrix}
\begin{pmatrix}
1\\ 1\\ 1
\end{pmatrix}\right]=
\begin{pmatrix}
0.3\\ 0.3\\ 0.3
\end{pmatrix}$\\\\

\indent $x^2 = \phi\left[
\begin{pmatrix}
2 & 2 & 2 & 2\\
2 & 2 & 2 & 2
\end{pmatrix}
\begin{pmatrix}
1\\ 0.3\\ 0.3 \\ 0.3
\end{pmatrix}\right]=
\begin{pmatrix}
3.8\\ 3.8
\end{pmatrix}$\\\\

\indent $x^3 = \phi\left[
\begin{pmatrix}
1 & 1 & 1\\
1 & 1 & 1
\end{pmatrix}
\begin{pmatrix}
1\\ 3.8\\ 3.8
\end{pmatrix}\right]=
\begin{pmatrix}
8.6 \\ 8.6
\end{pmatrix}$\\\\



\noindent \hrulefill \\



\noindent 11) $\delta^{(3)} = 
\begin{pmatrix}
8.6 \\ 8.6
\end{pmatrix} - 
\begin{pmatrix}
1 \\ 0
\end{pmatrix} = 
\begin{pmatrix}
7.6 \\ 8.6
\end{pmatrix}$\\\\

\indent $\delta^{(2)} = 
\begin{pmatrix}
0(1 - 0) \\ 3.8(1 - 3.8) \\ 3.8(1 - 3.8)
\end{pmatrix} \circ \left(
\begin{pmatrix}
1 & 1 \\
1 & 1 \\
1 & 1 
\end{pmatrix}
\begin{pmatrix}
7.6 \\ 8.6
\end{pmatrix} \right) = 
\begin{pmatrix}
0 \\ -172.368 \\ -172.368
\end{pmatrix}
$\\\\

\indent $\delta^{(1)} = 
\begin{pmatrix}
0(1 - 0) \\ 0.3(1 - 0.3) \\ 0.3(1 - 0.3) \\ 0.3(1 - 0.3)
\end{pmatrix} \circ \left(
\begin{pmatrix}
2 & 2 \\
2 & 2 \\
2 & 2 \\
2 & 2 
\end{pmatrix}
\begin{pmatrix}
-172.368 \\ -172.368
\end{pmatrix}\right) = 
\begin{pmatrix}
0 \\ -144.789 \\ -144.789 \\ -144.789
\end{pmatrix}
$\\



\noindent \hrulefill \\\pagebreak



\noindent 12) $\nabla^{(2)} = x^{(2)}(\delta^{(3)})^T = 
\begin{pmatrix}
1\\ 3.8\\ 3.8
\end{pmatrix}
[7.6, 8.6] = 
\begin{pmatrix}
7.6 & 8.6 \\
28.88 & 32.68 \\
28.88 & 32.68
\end{pmatrix}
$\\\\

\indent $\nabla^{(1)} = x^{(1)}(\delta^{(2)})^T = 
\begin{pmatrix}
1\\ 0.3\\ 0.3 \\ 0.3
\end{pmatrix}
[-172.368, -172.368] = 
\begin{pmatrix}
-172.368 & -172.368 \\
-51.71 & -51.71 \\
-51.71 & -51.71 \\
-51.71 & -51.71 
\end{pmatrix}
$\\\\

\indent $\nabla^{(0)} = x^{(0)}(\delta^{(1)})^T = 
\begin{pmatrix}
1\\ 1\\ 1
\end{pmatrix}
[-144.789, -144.789, -144.789] = 
\begin{pmatrix}
-144.789 & -144.789 & -144.789 \\
-144.789 & -144.789 & -144.789 \\
-144.789 & -144.789 & -144.789 
\end{pmatrix}
$\\



\noindent \hrulefill \\



\noindent 13) $\mathbb{W}^{2} \leftarrow \mathbb{W}^{2} - \rho\nabla^{(2)} = 
\begin{pmatrix}
1 & 1 \\
1 & 1 \\
1 & 1 
\end{pmatrix} - 
\begin{pmatrix}
7.6 & 8.6 \\
28.88 & 32.68 \\
28.88 & 32.68
\end{pmatrix} = 
\begin{pmatrix}
-6.6 & -7.6 \\
-27.88 & -31.68 \\
-27.88 & -31.68
\end{pmatrix}
$\\\\

\indent $\mathbb{W}^{1} \leftarrow \mathbb{W}^{1} - \rho\nabla^{(1)} = 
\begin{pmatrix}
2 & 2 \\
2 & 2 \\
2 & 2 \\
2 & 2 
\end{pmatrix} - 
\begin{pmatrix}
-172.368 & -172.368 \\
-51.71 & -51.71 \\
-51.71 & -51.71 \\
-51.71 & -51.71 
\end{pmatrix} = 
\begin{pmatrix}
174.368 & 174.368 \\
53.71 & 53.71 \\
53.71 & 53.71 \\
53.71 & 53.71 
\end{pmatrix}
$\\\\

\indent $\mathbb{W}^{0} \leftarrow \mathbb{W}^{0} - \rho\nabla^{(0)} = 
\begin{pmatrix}
0.1 & 0.1 & 0.1\\
0.1 & 0.1 & 0.1\\
0.1 & 0.1 & 0.1
\end{pmatrix} - 
\begin{pmatrix}
-144.789 & -144.789 & -144.789 \\
-144.789 & -144.789 & -144.789 \\
-144.789 & -144.789 & -144.789 
\end{pmatrix} = $\\
\begin{center}$
\begin{pmatrix}
144.889 & 144.889 & 144.889 \\
144.889 & 144.889 & 144.889 \\
144.889 & 144.889 & 144.889 
\end{pmatrix}$
\end{center}


\noindent \hrulefill \\





%\begin{figure}[htbp]
%\centerline{\includegraphics{Pics/ComS472_410.png}}
%\caption{Belief states recheable from initial 8 belief states.}
%\label{Belief states recheable from initial 8 belief states.}
%\end{figure}

\end{document}

















